\begin{cor}
    \label{cor:HellysTheorem}
    Let X be a \SeminormedSpace.
    Let, $x^{**} \in X^{**}$.
    Let $\{x_i^*\}_{i=1}^n \subset X^*$.
    Let and $\epsilon > 0$. 
    The following are true
    \begin{enumerate}[label=(\roman*), ref={\ref{cor:HellysTheorem}~\roman*}]
        \item 
        \label{cor:HellysTheorem:ThreeImpliesOne}
        There exists an $x_1 \in X$ 
        such that $\norm{x_1} \leq \norm{x^{**}}+\epsilon$ 
        and for $1 \leq i \leq n$, 
        $\ip{x_1,x_i^*} = \ip{x_i^*,x^{**}}$.  
        \item 
        \label{cor:HellysTheorem:ThreeImpliesTwo}
        There exists an $x_2 \in X$ 
        such that $\norm{x_2} \leq \norm{x^{**}}$ 
        and for $1 \leq i \leq n$, 
        $\abs{\ip{x_2,x_i^*}-\ip{x_i^*,x^{**}}} < \epsilon$. 
    \end{enumerate} 
    \begin{proof}[Proof of Both]
    For $1 \leq i \leq n$, define $\alpha_i = \ip{x_i^*, x^{**}}$. 
    Let $\{\beta_i\}_{i=1}^n \subset \bbC$. 
    Then, 
    \begin{align*}
    \abs{\sum\limits_{i=1}^n \beta_i \alpha_i}
    & = \abs{\sum\limits_{i=1}^n \beta_i \ip{x_i^*, x^**}}\\
    & = \abs{\ip{\sum\limits_{i=1}^n \beta_i x_i^*, x^{**}}}\\
    & \leq \norm{x^**} \norm{\sum\limits_{i=1}^n \beta_i x_i^*}
    \end{align*}
    Hence $\ref{thm:HellysTheorem:3}$ is satisfied with $\alpha_i=\ip{x_i^*, x^**}$ 
    and $M = \norm{x^{**}}$. 
    From an application of 
    $\ref{thm:HellysTheorem:3} \implies \ref{thm:HellysTheorem:2}$, 
    we conclude the existence of 
    $x_{1} \in X$ 
    with 
    $\ip{x_1, x_i^*} = \alpha_i = \ip{x_i^*, x^{**}}$ 
    and 
    $\norm{x_1} \leq \norm{x^**}+\epsilon$, 
    so \ref{cor:HellysTheorem:ThreeImpliesOne} holds.
    Also, from 
    $\ref{thm:HellysTheorem:3} \implies \ref{thm:HellysTheorem:1}$, 
    we conclude the existence of an 
    $x_2 \in X$ 
    satisfying
    \begin{align*}
        \abs{\ip{x_2, x_i^*} - \ip{x_i^*, x^{**}}} 
        & = \abs{\ip{x_2, x_i^*} - \alpha_i} \\
        & < \epsilon
    \end{align*}
    and $\norm{x_2} \leq \norm{x^{**}}$. 
    Hence \ref{cor:HellysTheorem:ThreeImpliesTwo} holds.
    \end{proof}
\end{cor} 

